theories/interop/prims_proto.v
@@ -1,0 +1,137 @@
+From Coq Require Import ssreflect.
+From stdpp Require Import strings gmap list.
+From iris.proofmode Require Import proofmode.
+From melocoton Require Import named_props.
+From melocoton.ml_lang Require Import lang_instantiation primitive_laws.
+From melocoton.interop Require Import basics_resources gctoken prims.
+
+Section PrimsProto.
+
+Context {hlc : has_lc}.
+Context {Σ : gFunctors}.
+Context `{!heapGS_ML Σ, !heapGS_C Σ}.
+Context `{!invGS_gen hlc Σ}.
+Context `{!wrapperGCtokGS Σ}.
+
+(* XXX? *)
+Notation mkPeML p T := ({| penv_prog := p; penv_proto := T |} : prog_environ ML_lang (_ : gFunctors)).
+
+Notation prim_proto := (prim -d> list C_intf.val -d> (C_intf.val -d> iPropO Σ) -d> iPropO Σ).
+Notation C_proto := (string -d> list C_intf.val -d> (C_intf.val -d> iPropO Σ) -d> iPropO Σ).
+Notation ML_proto := (string -d> list ML_lang.val -d> (ML_lang.val -d> iPropO Σ) -d> iPropO Σ).
+
+Definition proto_int2val : prim_proto := (λ p vl Φ,
+   ∃ θ z,
+     "HGC" ∷ GC θ ∗
+     "->" ∷ ⌜p = Pint2val⌝ ∗
+     "->" ∷ ⌜vl = [C_intf.LitV $ C_intf.LitInt $ z]⌝ ∗
+     "Cont" ∷ (∀ w, GC θ -∗ ⌜repr_lval θ (Lint z) w⌝ -∗ Φ w))%I.
+
+Definition proto_val2int : prim_proto := (λ p vl Φ,
+   ∃ θ w z,
+     "HGC" ∷ GC θ ∗
+     "->" ∷ ⌜p = Pval2int⌝ ∗
+     "->" ∷ ⌜vl = [ w ]⌝ ∗
+     "%Hrepr" ∷ ⌜repr_lval θ (Lint z) w⌝ ∗
+     "Cont" ∷ (GC θ -∗ Φ (C_intf.LitV $ C_intf.LitInt $ z)))%I.
+
+Definition proto_registerroot : prim_proto := (λ p vl Φ,
+   ∃ θ l v w,
+     "HGC" ∷ GC θ ∗
+     "->" ∷ ⌜p = Pregisterroot⌝ ∗
+     "->" ∷ ⌜vl = [ C_intf.LitV $ C_intf.LitLoc $ l ]⌝ ∗
+     "Hpto" ∷ l ↦C w ∗
+     "%Hrepr" ∷ ⌜repr_lval θ v w⌝ ∗
+     "Cont" ∷ (GC θ -∗ l ↦roots v -∗ Φ (C_intf.LitV $ C_intf.LitInt $ 0)))%I.
+
+Definition proto_unregisterroot : prim_proto := (λ p vl Φ,
+   ∃ θ l v,
+     "HGC" ∷ GC θ ∗
+     "->" ∷ ⌜p = Punregisterroot⌝ ∗
+     "->" ∷ ⌜vl = [ C_intf.LitV $ C_intf.LitLoc $ l ]⌝ ∗
+     "Hpto" ∷ l ↦roots v ∗
+     "Cont" ∷ (∀w, GC θ -∗ l ↦C w -∗ ⌜repr_lval θ v w⌝ -∗ Φ (C_intf.LitV $ C_intf.LitInt $ 0)))%I.
+
+Definition proto_modify : prim_proto := (λ p vl Φ,
+  ∃ θ w i v' w' γ mut tg vs,
+    "HGC" ∷ GC θ ∗
+    "->" ∷ ⌜p = Pmodify⌝ ∗
+    "->" ∷ ⌜vl = [ w; C_intf.LitV $ C_intf.LitInt $ i; w' ]⌝ ∗
+    "%Hreprw" ∷ ⌜repr_lval θ (Lloc γ) w⌝ ∗
+    "%Hptomut" ∷ ⌜vblock_access_le M mut⌝ ∗
+    "Hpto" ∷ γ ↦vblk[mut] (tg, vs) ∗
+    "%Hreprw'" ∷ ⌜repr_lval θ v' w'⌝ ∗
+    "%Hi1" ∷ ⌜0 ≤ i⌝%Z ∗
+    "%Hi2" ∷ ⌜i < length vs⌝%Z ∗
+    "Cont" ∷ (GC θ -∗
+              γ ↦vblk[mut] (tg, <[Z.to_nat i:=v']> vs) -∗
+              Φ (C_intf.LitV $ C_intf.LitInt $ 0)))%I.
+
+Definition proto_readfield : prim_proto := (λ p vl Φ,
+   ∃ θ w i γ dq m tg vs,
+     "HGC" ∷ GC θ ∗
+     "->" ∷ ⌜p = Preadfield⌝ ∗
+     "->" ∷ ⌜vl = [ w; C_intf.LitV $ C_intf.LitInt $ i ]⌝ ∗
+     "%Hreprw" ∷ ⌜repr_lval θ (Lloc γ) w⌝ ∗
+     "Hpto" ∷ γ ↦vblk[m]{dq} (tg, vs) ∗
+     "%Hi1" ∷ ⌜0 ≤ i⌝%Z ∗
+     "%Hi2" ∷ ⌜i < length vs⌝%Z ∗
+     "Cont" ∷ (∀ v' w', GC θ -∗
+                        γ ↦vblk[m]{dq} (tg, vs) -∗
+                        ⌜vs !! (Z.to_nat i) = Some v'⌝ -∗
+                        ⌜repr_lval θ v' w'⌝ -∗
+                        Φ w'))%I.
+
+Definition proto_alloc : prim_proto := (λ p vl Φ,
+   ∃ θ tg sz,
+     "HGC" ∷ GC θ ∗
+     "->" ∷ ⌜p = Palloc⌝ ∗
+     "->" ∷ ⌜vl = [ C_intf.LitV $ C_intf.LitInt $ vblock_tag_as_int $ tg; C_intf.LitV $ C_intf.LitInt $ sz ]⌝ ∗
+     "%Hsz" ∷ ⌜0 ≤ sz⌝%Z ∗
+     "Cont" ∷ (∀ θ' γ w, GC θ' -∗
+                         γ ↦fresh (tg, List.repeat (Lint 0) (Z.to_nat sz)) -∗
+                         ⌜repr_lval θ' (Lloc γ) w⌝ -∗
+                         Φ w))%I.
+
+Definition proto_callback (E : coPset) (T : ML_proto) : prim_proto := (λ p vl Φ,
+  ∃ θ w γ w' lv' v' f x e ψ,
+    "HGC" ∷ GC θ ∗
+    "->" ∷ ⌜p = Pcallback⌝ ∗
+    "->" ∷ ⌜vl = [ w; w' ]⌝ ∗
+    "%Hreprw" ∷ ⌜repr_lval θ (Lloc γ) w⌝ ∗
+    "Hclos" ∷ γ ↦clos (f, x, e) ∗
+    "%Hreprw'" ∷ ⌜repr_lval θ lv' w'⌝ ∗
+    "Hsim'" ∷ lv' ~~ v' ∗
+    "WPcallback" ∷ ▷ WP (App (Val (RecV f x e)) (Val v')) @ mkPeML ∅ T ; E {{ ψ }} ∗
+    "Cont" ∷ (∀ θ' vret lvret wret,
+                GC θ' -∗
+                ψ vret -∗
+                lvret ~~ vret -∗
+                ⌜repr_lval θ' lvret wret⌝ -∗
+                Φ wret))%I.
+
+(* non-callbacks primitives *)
+Definition proto_base_prims : prim_proto := (λ p vl Φ,
+    proto_int2val p vl Φ ∨ proto_val2int p vl Φ ∨ proto_registerroot p vl Φ ∨ proto_unregisterroot p vl Φ
+  ∨ proto_modify p vl Φ ∨ proto_readfield p vl Φ ∨ proto_alloc p vl Φ)%I.
+
+Definition proto_prims E T : prim_proto := (λ p vl Φ,
+  proto_base_prims p vl Φ ∨ proto_callback E T p vl Φ)%I.
+
+Lemma proto_prims_mask_mono E1 E2 T : E1 ⊆ E2 →
+  ∀ p vl Φ, proto_prims E1 T p vl Φ -∗ proto_prims E2 T p vl Φ.
+Proof.
+  iIntros (H p vl Φ) "[HL|HR]".
+  1: by iLeft.
+  iNamed "HR". iRight.
+  do 10 iExists _; unfold named.
+  iFrame. do 4 (iSplit; first done).
+  iNext. iApply @wp_mask_mono. 1: done.
+  iFrame.
+Qed.
+
+Definition proto_prims_in_C E (T : ML_proto) : C_proto := (λ f vs Φ,
+  ∃ p, ⌜is_prim f p⌝ ∗ proto_prims E T p vs Φ
+)%I.
+
+End PrimsProto.
