theories/interop/wp_simulation.v
@@ -9,8 +9,8 @@ From iris.base_logic.lib Require Import ghost_map ghost_var.
 From iris.proofmode Require Import proofmode.
 From melocoton.c_interface Require Import defs resources.
 From melocoton.ml_lang Require Import lang lang_instantiation primitive_laws.
-From melocoton.interop Require Import prims weakestpre
-  wp_utils wp_ext_call_laws wp_boundary_laws.
+From melocoton.interop Require Export prims weakestpre prims_proto.
+From melocoton.interop Require Import wp_ext_call_laws wp_boundary_laws wp_utils.
 Import Wrap.
 
 Section Simulation.
